Substantially improved the rep_omega tactic

floyd/val_lemmas.v
@@ -749,59 +749,113 @@ Ltac const_equation x :=
   let y := eval compute in x
    in exact (x = y).
 
-Transparent Archi.ptr64.
-Definition int_wordsize_eq : ltac:(const_equation Int.wordsize) := eq_refl.
-Definition int_zwordsize_eq : ltac:(const_equation Int.zwordsize) := eq_refl.
-Definition int_modulus_eq :  ltac:(const_equation Int.modulus) := eq_refl.
-Definition int_half_modulus_eq :  ltac:(const_equation Int.half_modulus) := eq_refl.
-Definition int_max_unsigned_eq :  ltac:(const_equation Int.max_unsigned) := eq_refl.
-Definition int_max_signed_eq :  ltac:(const_equation Int.max_signed) := eq_refl.
-Definition int_min_signed_eq :  ltac:(const_equation Int.min_signed) := eq_refl.
+Ltac Zground X :=
+  match X with
+  | Z0 => idtac
+  | Zpos ?y => Zground y
+  | Zneg ?y => Zground y 
+  | xH => idtac
+  | xO ?y => Zground y
+  | xI ?y => Zground y
+ end.
 
-Definition int64_wordsize_eq : ltac:(const_equation Int64.wordsize) := eq_refl.
-Definition int64_zwordsize_eq : ltac:(const_equation Int64.zwordsize) := eq_refl.
-Definition int64_modulus_eq :  ltac:(const_equation Int64.modulus) := eq_refl.
-Definition int64_half_modulus_eq :  ltac:(const_equation Int64.half_modulus) := eq_refl.
-Definition int64_max_unsigned_eq :  ltac:(const_equation Int64.max_unsigned) := eq_refl.
-Definition int64_max_signed_eq :  ltac:(const_equation Int64.max_signed) := eq_refl.
-Definition int64_min_signed_eq :  ltac:(const_equation Int64.min_signed) := eq_refl.
+Ltac pose_const_equation X :=
+ match goal with
+ | H: X = ?Y |- _ => Zground Y
+ | _ => let z := eval compute in X in assert (X = z) by reflexivity
+ end.
 
-Definition ptrofs_wordsize_eq : ltac:(const_equation Ptrofs.wordsize) := eq_refl.
-Definition ptrofs_zwordsize_eq : ltac:(const_equation Ptrofs.zwordsize) := eq_refl.
-Definition ptrofs_modulus_eq :  ltac:(const_equation Ptrofs.modulus) := eq_refl.
-Definition ptrofs_half_modulus_eq :  ltac:(const_equation Ptrofs.half_modulus) := eq_refl.
-Definition ptrofs_max_unsigned_eq :  ltac:(const_equation Ptrofs.max_unsigned) := eq_refl.
-Definition ptrofs_max_signed_eq :  ltac:(const_equation Ptrofs.max_signed) := eq_refl.
-Definition ptrofs_min_signed_eq :  ltac:(const_equation Ptrofs.min_signed) := eq_refl.
-Opaque Archi.ptr64.
+Ltac perhaps_post_const_equation X :=
+ lazymatch goal with 
+ | H: context [X] |- _ => pose_const_equation X
+ | H:= context [X] |- _ => pose_const_equation X
+ | |- context [X] => pose_const_equation X
+ | |- _ => idtac
+ end.
+
+Ltac pose_const_equations L :=
+ match L with
+ | ?X :: ?Y => perhaps_post_const_equation X; pose_const_equations Y
+ | nil => idtac
+ end.
+
+Ltac register_omega_constants := constr:(@nil Z).
+
+Import ListNotations.
+
+Ltac pose_standard_const_equations :=
+pose_const_equations
+  [
+  Int.zwordsize; Int.modulus; Int.half_modulus; Int.max_unsigned; Int.max_signed; Int.min_signed;
+  Int64.zwordsize; Int64.modulus; Int64.half_modulus; Int64.max_unsigned; Int64.max_signed; Int64.min_signed;
+  Ptrofs.zwordsize; Ptrofs.modulus; Ptrofs.half_modulus; Ptrofs.max_unsigned; Ptrofs.max_signed; Ptrofs.min_signed;
+  Byte.min_signed; Byte.max_signed; Byte.max_unsigned; Byte.modulus
+  ];
+ pose_const_equations [Int.wordsize; Int64.wordsize; Ptrofs.wordsize];
+ pose_const_equations register_omega_constants.
+
+Definition Zlength' := @Zlength.
+
+Lemma Zlength_nonneg:
+ forall {A} (l: list A), 0 <= Zlength l.
+Proof.
+intros. rewrite Zlength_correct. omega.
+Qed.
+
+Ltac pose_Zlength_nonneg1 A :=
+     lazymatch goal with
+      | H:  0 <= Zlength A |- _ => idtac
+      | H:  0 <= Zlength A /\ _ |- _ => idtac
+      | |- _ => pose proof (Zlength_nonneg A)
+     end;  change (Zlength A) with (Zlength' _ A) in *.
+
+Ltac pose_Zlength_nonneg :=
+ repeat
+  match goal with
+  | |- context [Zlength ?A] => pose_Zlength_nonneg1 A
+  | H: context [Zlength ?A] |- _ => pose_Zlength_nonneg1 A
+  | H:= context [Zlength ?A] |- _ => pose_Zlength_nonneg1 A
+ end;
+  unfold Zlength' in *.
+
+Ltac pose_lemma F F' A L :=
+  match type of (L A) with ?T =>
+     lazymatch goal with
+      | H:  T |- _ => idtac
+      | H:  T /\ _ |- _ => idtac
+      | |- _ => pose proof (L A)
+     end;  change (F A) with (F' A) in *
+  end.
+
+Ltac pose_lemmas F F' L :=
+ repeat
+  match goal with
+  | |- context [F ?A] => pose_lemma F F' A L
+  | H: context [F ?A] |- _ => pose_lemma F F' A L
+ | H:= context [F ?A] |- _ => pose_lemma F F' A L
+ end;
+  unfold F' in *.
+
+Definition byte_unsigned' := Byte.unsigned.
+Definition byte_signed' := Byte.signed.
+Definition int_unsigned' := Int.unsigned.
+Definition int_signed' := Int.signed.
+Definition int64_unsigned' := Int64.unsigned.
+Definition int64_signed' := Int64.signed.
+Definition ptrofs_unsigned' := Ptrofs.unsigned.
 
 Ltac rep_omega := 
-   pose proof int_wordsize_eq;
-   pose proof int_zwordsize_eq;
-   pose proof int_modulus_eq;
-   pose proof int_half_modulus_eq;
-   pose proof int_max_unsigned_eq;
-   pose proof int_max_signed_eq;
-   pose proof int_min_signed_eq;
- 
-   pose proof int64_wordsize_eq;
-   pose proof int64_zwordsize_eq;
-   pose proof int64_modulus_eq;
-   pose proof int64_half_modulus_eq;
-   pose proof int64_max_unsigned_eq;
-   pose proof int64_max_signed_eq;
-   pose proof int64_min_signed_eq;
- 
-   pose proof ptrofs_wordsize_eq;
-   pose proof ptrofs_zwordsize_eq;
-   pose proof ptrofs_modulus_eq;
-   pose proof ptrofs_half_modulus_eq;
-   pose proof ptrofs_max_unsigned_eq;
-   pose proof ptrofs_max_signed_eq;
-   pose proof ptrofs_min_signed_eq;
-
-   unfold repable_signed in *;
-   omega.
+  unfold repable_signed in *;
+  pose_Zlength_nonneg;
+  pose_lemmas Byte.unsigned byte_unsigned' Byte.unsigned_range;
+  pose_lemmas Byte.signed byte_signed' Byte.signed_range;
+  pose_lemmas Int.unsigned int_unsigned' Int.unsigned_range;
+  pose_lemmas Int.signed int_signed' Int.signed_range;
+  pose_lemmas Int64.unsigned int64_unsigned' Int64.unsigned_range;
+  pose_lemmas Int64.signed int64_unsigned' Int64.signed_range;
+  pose_lemmas Ptrofs.unsigned ptrofs_unsigned' Ptrofs.unsigned_range;
+  pose_standard_const_equations;
+ omega.
 
 Ltac repable_signed := 
   idtac "Warning: repable_signed is deprecated;  use rep_omega"; rep_omega.
